src/examplelang/adequacy.v
@@ -1,0 +1,51 @@
+From ITree Require Import ITree Recursion RecursionFacts InterpFacts TranslateFacts Eqit.
+From iris Require Import invariants ghost_map.
+From iris.proofmode Require Import proofmode.
+From iris.bi Require Import weakestpre.
+From iris.itree Require Import wpi ub itree choice state step handler void heap.
+From iris.itree.threadpool Require Import ctrace handler interleaving.
+From iris.itree.examplelang Require Import lang program_logic.
+
+(** An execution outcome of a ExampleLang program. *)
+Definition Outcome R : Type :=
+  (heap.heap val * (R + last_thread_killed + ub_crash)).
+(** An execution of a ExampleLang program. *)
+Definition Execution R : Type :=
+  itree voidE (Outcome R).
+
+Definition examplelang_irel {R} (σ : heap.heap val) (n : option nat) (t : itree exampleE R)
+  (te : Execution R) : Prop :=
+  ∃ t1 t2 t3,
+    threadpool_irel t t1 ∧
+    ub_irel t1 t2 ∧
+    state_irel σ t2 t3 ∧
+    demonic_irel (insert_voidE t3) te.
+
+Section adequacy.
+  Context {Σ} `{!invGS Σ} `{!exampleHGS Σ}.
+
+  Lemma wp_adequacy_irel R t σ te (Φ : R → iProp Σ) n :
+    examplelang_irel σ n t te →
+    state_interp σ -∗
+    WPi t @ exampleH; ⊤ {{ Φ }} -∗
+    |={⊤, ∅}=> ∃ x, ⌜te ≈ Ret x⌝ ∗
+      match x with
+      | (_, inr UbCrash) => |={∅, ⊤}=> False
+      | (σ, inl (inl v)) => |={∅, ⊤}=> state_interp σ ∗ Φ v
+      | (σ, inl (inr LastThreadKilled)) => |={∅, ⊤}=> state_interp σ
+      end.
+  Proof.
+    iIntros ((?&?&?&?&->&?&?)) "Hs Hwp".
+    iDestruct (threadpool_adequacy with "Hwp") as "Hwp"; [done|].
+    iDestruct (ub_adequacy with "Hwp") as "Hwp"; [done|].
+    iDestruct (heap_adequacy with "Hs Hwp") as "Hwp"; [done|].
+    rewrite -wpi_clear_mask. iMod "Hwp".
+    iDestruct (wpi_insert_voidE with "Hwp") as "Hwp".
+    iDestruct (demonic_adequacy with "Hwp") as "Hwp"; [done|].
+    iApply void_adequacy_empty.
+    iApply wpi_wand; last done.
+    iIntros (?) "HΦ". repeat case_match; eauto.
+    - by iMod "HΦ" as "[$ _]".
+    - by iMod "HΦ" as "[_ $]".
+  Qed.
+End adequacy.
